@@ -401,6 +401,7 @@ import Xv6.ConsoleintrGhost
 import Xv6.ConsoleintrParts
 import Xv6.ConsoleintrArms
 import Xv6.ConsoleintrKill
+import Xv6.ConsolereadGhost
 import Xv6.ProofConsoleintr
 import Xv6.LinkConsoleintr
 import Xv6.LinkUartintr
